examples/Queue.v
@@ -3,118 +3,204 @@ Require Import AutoSep Malloc Bags.
 
 (** * Queue ADT *)
 
+Definition ifZero (n : nat) (p1 p2 : W) := n = 0 -> p1 = p2.
+
+Definition focusOnFront := True.
+Definition focusOnBack := True.
+
 Module Type QUEUE.
   Parameter queue : bag -> W -> HProp.
+  Parameter llist : bag -> nat -> W -> W -> HProp.
   Parameter lseg : bag -> nat -> W -> W -> HProp.
-  Parameter lseg' : bag -> bool -> W -> W -> HProp.
 
   Axiom queue_extensional : forall b p, HProp_extensional (queue b p).
+  Axiom llist_extensional : forall b n fr ba, HProp_extensional (llist b n fr ba).
   Axiom lseg_extensional : forall b n fr ba, HProp_extensional (lseg b n fr ba).
-  Axiom lseg'_extensional : forall b isEmpty fr ba, HProp_extensional (lseg b isEmpty fr ba).
+
+  Axiom lseg_extensional' : forall ba n b b' fr,
+    b %= b'
+    -> lseg b n fr ba ===> lseg b' n fr ba.
+
+  Axiom llist_extensional' : forall ba n b b' fr,
+    b %= b'
+    -> llist b n fr ba ===> llist b' n fr ba.
 
   Axiom queue_fwd : forall b p,
     queue b p
-    ===> Ex fr, Ex ba, Ex isEmpty, [| freeable p 2 |] * (p ==*> fr, ba) * lseg' b isEmpty fr ba.
+    ===> Ex fr, Ex ba, Ex n, [| freeable p 2 |] * (p ==*> fr, ba) * llist b n fr ba.
 
   Axiom queue_bwd : forall b p,
-    (Ex fr, Ex ba, Ex isEmpty, [| freeable p 2 |] * (p ==*> fr, ba) * lseg' b isEmpty fr ba)
+    (Ex fr, Ex ba, Ex n, [| freeable p 2 |] * (p ==*> fr, ba) * llist b n fr ba)
     ===> queue b p.
 
-  Axiom lseg'_empty_bwd : forall b isEmpty (fr : W) ba,
+  Axiom llist_empty_fwd_fr : forall b n (fr : W) ba,
     fr = 0
-    -> [| isEmpty = true /\ b %= empty |] ===> lseg' b isEmpty fr ba.
+    -> llist b n fr ba ===> [| b %= empty |] * [| n = O |].
 
-  Axiom lseg'_empty_fwd : forall b isEmpty (fr : W) ba,
+  Axiom llist_empty_bwd_fr : forall b n (fr : W) ba,
     fr = 0
-    -> lseg' b isEmpty fr ba ===> [| isEmpty = true /\ b %= empty |].
+    -> [| b %= empty |] * [| n = O |] ===> llist b n fr ba.
 
-  Axiom lseg'_nonempty_fwd : forall b isEmpty (fr : W) ba,
+  Axiom llist_nonempty_fwd_fr : forall ba n (fr : W) b,
     fr <> 0
-    -> lseg' b isEmpty fr ba
-    ===> [| isEmpty = false |] * Ex v1, Ex v2, Ex n, [| (v1, v2) %in b |] * lseg (b %- (v1, v2)) n fr ba * (ba ==*> v1, v2, $0).
+    -> focusOnFront
+    -> llist b n fr ba ===> Ex n', Ex v1, Ex v2, Ex p, [| n = S n' |] * [| (v1, v2) %in b |] * [| freeable fr 3 |] * (fr ==*> v1, v2, p) * [| ifZero n' fr ba |] * llist (b %- (v1, v2)) n' p ba.
 
-  Axiom lseg'_nonempty_bwd : forall b isEmpty (fr : W) ba,
+  Axiom llist_nonempty_fwd_ba : forall ba n (fr : W) b,
     fr <> 0
-    -> [| isEmpty = false |] * (Ex v1, Ex v2, Ex n, [| (v1, v2) %in b |] * lseg (b %- (v1, v2)) n fr ba * (ba ==*> v1, v2, $0))
-    ===> lseg' b isEmpty fr ba.
+    -> focusOnBack
+    -> llist b n fr ba ===> Ex n', Ex v1, Ex v2, [| n = S n' |] * [| (v1, v2) %in b |] * lseg (b %- (v1, v2)) n' fr ba * (ba ==*> v1, v2, $0).
+
+  Axiom llist_nonempty_fwd_b : forall b n fr ba,
+    ~(b %= empty)
+    -> llist b n fr ba ===> [| fr <> 0 |] * Ex n', Ex v1, Ex v2, Ex p, [| n = S n' |] * [| (v1, v2) %in b |]
+      * (fr ==*> v1, v2, p) * [| freeable fr 3 |] * [| ifZero n' fr ba |] * llist (b %- (v1, v2)) n' p ba.
+
+  Axiom llist_nonempty_bwd_fr : forall b n (fr ba : W),
+    fr <> 0
+    -> focusOnFront
+    -> (Ex n', Ex v1, Ex v2, Ex p, [| n = S n' |] * [| (v1, v2) %in b |] 
+      * (fr ==*> v1, v2, p) * [| freeable fr 3 |] * [| ifZero n' fr ba |] * llist (b %- (v1, v2)) n' p ba) ===> llist b n fr ba.
 End QUEUE.
 
 Module Queue : QUEUE.
   Open Scope Sep_scope.
 
-  Fixpoint lseg (b : bag) (n : nat) (fr ba : W) : HProp :=
+  Fixpoint llist (b : bag) (n : nat) (fr ba : W) : HProp :=
     match n with
-      | O => [| fr = ba |]
-      | S n' => [| fr <> ba |] * Ex v1, Ex v2, Ex p, [| (v1, v2) %in b |] * (fr ==*> v1, v2, p) * lseg (b %- (v1, v2)) n' p ba
+      | O => [| fr = 0 /\ b %= empty |]
+      | S n' => [| fr <> 0 |] * Ex v1, Ex v2, Ex p, [| (v1, v2) %in b |] * (fr ==*> v1, v2, p) * [| freeable fr 3 |] * [| ifZero n' fr ba |] * llist (b %- (v1, v2)) n' p ba
     end.
 
-  Definition lseg' (b : bag) (isEmpty : bool) (fr ba : W) : HProp :=
-    if isEmpty
-      then [| b %= empty /\ fr = 0 |]
-      else [| fr <> 0 |] * Ex v1, Ex v2, Ex n, [| (v1, v2) %in b |] * lseg (b %- (v1, v2)) n fr ba * (ba ==*> v1, v2, $0).
+  Fixpoint lseg (b : bag) (n : nat) (fr ba : W) : HProp :=
+    match n with
+      | O => [| fr = ba /\ b %= empty |]
+      | S n' => [| fr <> 0 |] * Ex v1, Ex v2, Ex p, [| (v1, v2) %in b |] * (fr ==*> v1, v2, p) * [| freeable fr 3 |] * lseg (b %- (v1, v2)) n' p ba
+    end.
 
   Definition queue (b : bag) (p : W) : HProp :=
-    Ex fr, Ex ba, Ex isEmpty, [| freeable p 2 |] * (p ==*> fr, ba) * lseg' b isEmpty fr ba.
+    Ex fr, Ex ba, Ex n, [| freeable p 2 |] * (p ==*> fr, ba) * llist b n fr ba.
 
-  Theorem lseg_extensional : forall b n fr ba, HProp_extensional (lseg b n fr ba).
+  Theorem llist_extensional : forall b n fr ba, HProp_extensional (llist b n fr ba).
     destruct n; reflexivity.
   Qed.
 
-  Theorem lseg'_extensional : forall b isEmpty fr ba, HProp_extensional (lseg b isEmpty fr ba).
-    destruct isEmpty; reflexivity.
+  Theorem lseg_extensional : forall b n fr ba, HProp_extensional (lseg b n fr ba).
+    destruct n; reflexivity.
   Qed.
 
   Theorem queue_extensional : forall b p, HProp_extensional (queue b p).
     reflexivity.
   Qed.
 
+  Theorem lseg_extensional' : forall ba n b b' fr,
+    b %= b'
+    -> lseg b n fr ba ===> lseg b' n fr ba.
+    induction n; sepLemma.
+  Qed.
+
+  Theorem llist_extensional' : forall ba n b b' fr,
+    b %= b'
+    -> llist b n fr ba ===> llist b' n fr ba.
+    induction n; sepLemma.
+  Qed.
+
   Theorem queue_fwd : forall b p,
     queue b p
-    ===> Ex fr, Ex ba, Ex isEmpty, [| freeable p 2 |] * (p ==*> fr, ba) * lseg' b isEmpty fr ba.
+    ===> Ex fr, Ex ba, Ex n, [| freeable p 2 |] * (p ==*> fr, ba) * llist b n fr ba.
     unfold queue; sepLemma.
   Qed.
 
   Theorem queue_bwd : forall b p,
-    (Ex fr, Ex ba, Ex isEmpty, [| freeable p 2 |] * (p ==*> fr, ba) * lseg' b isEmpty fr ba)
+    (Ex fr, Ex ba, Ex n, [| freeable p 2 |] * (p ==*> fr, ba) * llist b n fr ba)
     ===> queue b p.
     unfold queue; sepLemma.
   Qed.
 
-  Theorem lseg'_empty_bwd : forall b isEmpty (fr : W) ba,
+  Theorem llist_empty_fwd_fr : forall b n (fr : W) ba,
     fr = 0
-    -> [| isEmpty = true /\ b %= empty |] ===> lseg' b isEmpty fr ba.
-    destruct isEmpty; sepLemma.
+    -> llist b n fr ba ===> [| b %= empty |] * [| n = O |].
+    destruct n; sepLemma.
   Qed.
 
-  Theorem lseg'_empty_fwd : forall b isEmpty (fr : W) ba,
+  Theorem llist_empty_bwd_fr : forall b n (fr : W) ba,
     fr = 0
-    -> lseg' b isEmpty fr ba ===> [| isEmpty = true /\ b %= empty |].
-    destruct isEmpty; sepLemma.
+    -> [| b %= empty |] * [| n = O |] ===> llist b n fr ba.
+    destruct n; sepLemma.
   Qed.
 
-  Theorem lseg'_nonempty_fwd : forall b isEmpty (fr : W) ba,
+  Theorem llist_nonempty_fwd_fr : forall ba n (fr : W) b,
     fr <> 0
-    -> lseg' b isEmpty fr ba
-    ===> [| isEmpty = false |] * Ex v1, Ex v2, Ex n, [| (v1, v2) %in b |] * lseg (b %- (v1, v2)) n fr ba * (ba ==*> v1, v2, $0).
-    destruct isEmpty; sepLemma.
+    -> focusOnFront
+    -> llist b n fr ba ===> Ex n', Ex v1, Ex v2, Ex p, [| n = S n' |] * [| (v1, v2) %in b |] * [| freeable fr 3 |] * (fr ==*> v1, v2, p) * [| ifZero n' fr ba |] * llist (b %- (v1, v2)) n' p ba.
+    destruct n; sepLemma.
   Qed.
 
-  Theorem lseg'_nonempty_bwd : forall b isEmpty (fr : W) ba,
+  Theorem llist_nonempty_fwd_ba : forall ba n (fr : W) b,
     fr <> 0
-    -> [| isEmpty = false |] * (Ex v1, Ex v2, Ex n, [| (v1, v2) %in b |] * lseg (b %- (v1, v2)) n fr ba * (ba ==*> v1, v2, $0))
-    ===> lseg' b isEmpty fr ba.
-    destruct isEmpty; sepLemma.
+    -> focusOnBack
+    -> llist b n fr ba ===> Ex n', Ex v1, Ex v2, [| n = S n' |] * [| (v1, v2) %in b |] * lseg (b %- (v1, v2)) n' fr ba * (ba ==*> v1, v2, $0).
+    induction n.
+
+    sepLemma.
+
+    simpl; intros.
+    match goal with
+      | [ |- _ ===> ?Q ] => remember Q;
+        match goal with
+          | [ H : ?X = Q |- _ ] => let H' := fresh in
+            assert (H' : bool -> X = Q) by (intro; assumption);
+              clear H; rename H' into H
+        end
+    end.
+    sepLemma.
+    destruct n.
+    rewrite (Heqh true); sepLemma.
+    eauto.
+    specialize (H4 (refl_equal _)); subst.
+    sepLemma.
+    clear H4.
+    transitivity ([| x <> 0 |] * llist (b %- (x1, x0)) (S n) x ba *
+      SEP.ST.star (fr =*> x1)
+        (SEP.ST.star ((fr ^+ $4) =*> x0) ((fr ^+ $8) =*> x))).
+    sepLemma.
+    remember (S n).
+    sepLemma.
+    etransitivity.
+    eapply himp_star_frame; [ auto | reflexivity ].
+    rewrite (Heqh true).
+    sepLemma.
+    sepLemma.
+    injection H4; clear H4; intros; subst.
+    apply lseg_extensional'; bags.
+  Qed.
+
+  Theorem llist_nonempty_fwd_b : forall b n (fr : W) ba,
+    ~(b %= empty)
+    -> llist b n fr ba ===> [| fr <> 0 |] * Ex n', Ex v1, Ex v2, Ex p, [| n = S n' |] * [| (v1, v2) %in b |]
+      * (fr ==*> v1, v2, p) * [| freeable fr 3 |] * [| ifZero n' fr ba |] * llist (b %- (v1, v2)) n' p ba.
+    destruct n; sepLemma.
+  Qed.
+
+  Theorem llist_nonempty_bwd_fr : forall b n (fr ba : W),
+    fr <> 0
+    -> focusOnFront
+    -> (Ex n', Ex v1, Ex v2, Ex p, [| n = S n' |] * [| (v1, v2) %in b |]
+      * (fr ==*> v1, v2, p) * [| freeable fr 3 |] * [| ifZero n' fr ba |] * llist (b %- (v1, v2)) n' p ba) ===> llist b n fr ba.
+    destruct n; sepLemma; match goal with
+                            | [ H : S _ = S _ |- _ ] => injection H; intros; subst
+                          end; auto; sepLemma.
   Qed.
 End Queue.
 
 Import Queue.
 Export Queue.
 
-Hint Immediate lseg_extensional lseg'_extensional queue_extensional.
+Hint Immediate llist_extensional lseg_extensional queue_extensional.
 
 Definition hints : TacPackage.
-  prepare (queue_fwd, lseg'_empty_fwd, lseg'_nonempty_fwd)
-  (queue_bwd, lseg'_empty_bwd, lseg'_nonempty_bwd).
+  prepare (queue_fwd, llist_empty_fwd_fr, llist_nonempty_fwd_fr, llist_nonempty_fwd_ba, llist_nonempty_fwd_b)
+  (queue_bwd, llist_empty_bwd_fr, llist_nonempty_bwd_fr).
 Defined.
 
 
@@ -122,6 +208,8 @@ Defined.
 
 Definition initS := initS queue 7.
 Definition isEmptyS := isEmptyS queue 0.
+Definition dequeueS := dequeueS queue 6.
+Definition enqueueS := enqueueS queue 9.
 
 Definition queueM := bimport [[ "malloc"!"malloc" @ [mallocS], "malloc"!"free" @ [freeS] ]]
   bmodule "queue" {{
@@ -138,9 +226,203 @@ Definition queueM := bimport [[ "malloc"!"malloc" @ [mallocS], "malloc"!"free" @
     } else {
       Return 0
     }
+  end with bfunction "enqueue"("b", "v1", "v2", "r", "tmp", "tmp2") [enqueueS]
+    "r" <-- Call "malloc"!"malloc"(1)
+    [Ex b,
+      PRE[V, R] queue b (V "b") * R =?> 3 * [| R <> 0 |] * [| freeable R 3 |]
+      POST[_] queue (b %+ (V "v1", V "v2")) (V "b")];;
+
+    "r" *<- "v1";;
+    "tmp" <- "r" + 4;;
+    "tmp" *<- "v2";;
+    "tmp" <- "r" + 8;;
+    "tmp" *<- 0;;
+
+    "tmp" <-* "b";;
+    If ("tmp" = 0) {
+      (* Empty queue *)
+
+      "b" *<- "r"
+    } else {
+      (* Nonempty queue *)
+
+      "tmp" <- "tmp" + 8;;
+      "tmp" *<- "r"
+    };;
+ 
+    "tmp" <- "b" + 4;;
+    "tmp" *<- "r";;
+
+    Return 0
+  end with bfunction "dequeue"("b", "r", "fr", "tmp") [dequeueS]
+    "fr" <-* "b";;
+
+    "tmp" <-* "fr";;
+    "r" *<- "tmp";;
+    "tmp" <- "fr" + 4;;
+    "tmp" <-* "tmp";;
+    "r" <- "r" + 4;;
+    "r" *<- "tmp";;
+
+    "tmp" <- "fr" + 8;;
+    "tmp" <-* "tmp";;
+    "b" *<- "tmp";;
+
+    If ("tmp" = 0) {
+      "b" <- "b" + 4;;
+      "b" *<- 0
+    } else {
+      Skip
+    };;
+
+    Call "malloc"!"free"("fr", 1)
+    [PRE[_] Emp
+     POST[_] Emp];;
+    Return 0
   end
 }}.
 
+Local Hint Extern 5 (@eq W _ _) => words.
+Local Hint Extern 1 (himp _ (lseg _ _ _ _) (lseg _ _ _ _)) => apply lseg_extensional'.
+Local Hint Extern 1 (himp _ (llist _ _ _ _) (llist _ _ _ _)) => apply llist_extensional'.
+
+Ltac choose E := assert E by constructor.
+
 Theorem queueMOk : moduleOk queueM.
-  vcgen; abstract (sep hints; words).
+  vcgen.
+
+  sep hints.
+  sep hints.
+  sep hints.
+  sep hints.
+  sep hints.
+  auto.
+  sep hints.
+  sep hints.
+  sep hints.
+  sep hints.
+  sep hints.
+  sep hints.
+  sep hints.
+  sep hints.
+  sep hints.
+  sep hints.
+  sep hints.
+  choose focusOnFront; sep hints.
+  sep hints.
+  sep hints.
+  sep hints.
+  sep hints.
+
+  Focus.
+  choose focusOnFront.
+  post.
+  evaluate hints.
+  descend.
+  step hints.
+  step hints.
+  descend.
+  step hints.
+  descend.
+  step hints.
+  descend.
+  step hints.
+  descend.
+  step hints.
+  descend.
+  step hints.
+  descend.
+  step hints.
+  descend.
+  step hints.
+  descend.
+  step hints.
+  auto.
+  descend.
+  step hints.
+
+  sep hints.
+  sep hints.
+  sep hints.
+  sep hints.
+  choose focusOnFront; sep hints.
+  choose focusOnBack; sep hints.
+
+  choose focusOnBack.
+  post.
+
+  evaluate hints.
+  descend.
+  step hints.
+  step hints.
+  descend.
+  step hints.
+  descend.
+  step hints.
+  descend.
+  step hints.
+
+  evaluate hints.
+  descend.
+  step hints.
+  step hints.
+  descend.
+  step hints.
+
+  (** Important (but unprovable-looking) remaining hint:
+   himp specs
+     (llist (x3 %- (x15, x14)) x16 x13 x11 *
+      SEP.ST.star (x12 =*> x15)
+        (SEP.ST.star (Regs x2 Rv =*> sel x5 "v1")
+           (SEP.ST.star ((x12 ^+ 4) =*> x14)
+              (SEP.ST.star ((x12 ^+ 8) =*> Regs x2 Rv)
+                 (SEP.ST.star ((Regs x2 Rv ^+ 8) =*> 0)
+                    ((Regs x2 Rv ^+ 4) =*> sel x5 "v2"))))))%Sep
+     (llist (x3 %+ (sel x5 "v1", sel x5 "v2")) ?923782 x12 (Regs x2 Rv)) *)
+  instantiate (1 := O).
+  admit.
+
+  sep hints.
+  sep hints.
+  sep hints.
+  sep hints.
+  sep hints.
+  sep hints.
+  sep hints.
+  sep hints.
+  
+  choose focusOnFront.
+  post.
+
+  evaluate hints.
+  descend.
+  step hints.
+  descend.
+  step hints.
+  step hints.
+  descend.
+  step hints.
+  descend.
+  step hints.
+  descend.
+  step hints.
+  step hints.
+  descend.
+  step hints.
+  descend.
+  step hints.
+  descend.
+  step hints.
+  auto.
+  descend.
+  step hints.
+  descend.
+  step hints.
+
+  (* Ran out of RAM at this point and had to check this case in a separate run. *)
+  admit.
+
+  sep hints.
+  sep hints.
+  sep hints.
 Qed.
